Fix test

Source/IntegrationTests/TestFiles/LitTests/LitTest/ast/expressions/statementExpressions.dfy
@@ -1,16 +1,28 @@
-// RUN: %verify --type-system-refresh --allow-axioms --bprint:%t.bpl --isolate-assertions --boogie "/printPruned:%S/pruned" %s > %t
+// RUN: ! %verify --type-system-refresh --allow-axioms --bprint:%t.bpl --isolate-assertions %s > %t
 // RUN: %diff "%s.expect" "%t"
 
-function StmtExprValueAndEnsures(): int
-  ensures ValueAndEnsures() == 42 
+function StatementExpressionValueAndEnsures(): int
+  ensures StatementExpressionValueAndEnsures() == 42 
 {
   assert true; 42
 }
 
-function ExpressionWFVersusFunctionEnsures(): int 
+function StatementExpressionAssumeAndFunctionEnsures(): int 
   ensures 10 == 11 // no error, since the statement expression can be used for the ensures clause
 {
   assume false; 10
+}
+
+function StatementExpressionAndSubsetResult(): nat 
+  // no error, since the statement expression can be used for the return type subset constraint
+{
+  assume -1 > 0; -1
+}
+
+method StatementExpressionAndSubsetLocal() 
+  // no error, since the statement expression can be used for the return type subset constraint
+{
+  var x: nat := assume -1 > 0; -1;
 }
 
 function ExpressionWFAndLet(): int 
@@ -20,7 +32,7 @@ function ExpressionWFAndLet(): int
   x
 }
 
-method Bar() {
+method StatementExpressionAssumeDoesNotEscapeExpression() {
   var x := assume false; 3;
   assert false; // error
 }
